spec and fixes, etc

theories/instantiation.v
@@ -275,11 +275,15 @@ Definition dummy_mem := {|
   mem_max_opt := None
 |}.
 
+(* Originally using the write_bytes operation to keep memory implementation parametric, albeit a less convenient definition to use. However, there's an edge case in the bound check that renders its behaviour slightly off when offset is oob with an empty initialiser payload, so replaced by the following version. *)
 Definition init_mem (s : store_record) (inst : instance) (d_ind : N) (d : module_data) : store_record :=
   let m_ind := List.nth (match d.(moddata_data) with Mk_memidx i => i end) inst.(inst_memory) 0 in
   let mem := List.nth m_ind s.(s_mems) dummy_mem in
-  let mem'_opt := operations.write_bytes mem d_ind (List.map bytes.compcert_byte_of_byte d.(moddata_init)) in
-  let mems' := match mem'_opt with None => s.(s_mems) | Some mem' => insert_at mem' m_ind s.(s_mems) end in
+  let d_pay := List.map bytes.compcert_byte_of_byte d.(moddata_init) in
+  let mem'_e := List.app (List.firstn d_ind mem.(mem_data).(ml_data)) (List.app d_pay (List.skipn (d_ind + length d_pay) mem.(mem_data).(ml_data))) in
+(*  let mem'_opt := operations.write_bytes mem d_ind (List.map bytes.compcert_byte_of_byte d.(moddata_init)) in
+  let mems' := match mem'_opt with None => s.(s_mems) | Some mem' => insert_at mem' m_ind s.(s_mems) end in*)
+  let mems' := insert_at {| mem_data := {| ml_data := mem'_e; ml_init := mem.(mem_data).(ml_init) |}; mem_max_opt := mem.(mem_max_opt) |} m_ind s.(s_mems) in
   {| s_funcs := s.(s_funcs);
      s_tables := s.(s_tables);
      s_mems := mems';
